Add make_blob_coupon equivalence proof

wasm-proofs/Wasm-Proof/Host.thy
@@ -13,6 +13,12 @@ and
 
 definition type0 :: "tf" where [simp]:
   "type0 = Tf [(T_ref T_ext_ref), (T_ref T_ext_ref)] [(T_num T_i32)]"
+definition type1 :: "tf" where [simp]:
+  "type1 = Tf [(T_ref T_ext_ref)] [(T_num T_i32)]"
+definition type2 :: "tf" where [simp]:
+  "type2 = Tf [(T_ref T_ext_ref)] [(T_ref T_ext_ref)]"
+definition type3 :: "tf" where [simp]:
+  "type3 = Tf [(T_ref T_ext_ref), (T_ref T_ext_ref)] [(T_ref T_ext_ref)]"
 
 (* functions and lemmas for translating between isabelle bool and wasm i32*)
 fun bool_to_i32 :: "bool \<Rightarrow> i32" where
@@ -48,6 +54,10 @@ lemma bool_to_i32_false:
 
 (* Fixpoint APIs exposed to Wasm modules *)
 consts fixpoint_is_equal :: host_func
+consts fixpoint_is_storage_coupon_api :: host_func
+consts fixpoint_get_coupon_lhs :: host_func
+consts fixpoint_get_coupon_rhs :: host_func
+consts fixpoint_create_eq_coupon :: host_func
 
 axiomatization where
   (* We are stating here that the exposed fixpoint_is_equal is the same as
@@ -56,18 +66,28 @@ axiomatization where
   "host_func_apply_impl s type0 fixpoint_is_equal 
   [(V_ref (ConstRefExtern r1)), (V_ref (ConstRefExtern r2))]
   = Some (s, [V_num (ConstInt32 (bool_to_i32 (is_equal (to_handle r1) (to_handle r2))))])"
+and
+  fixpoint_is_storage_coupon_api_impl:
+  "host_func_apply_impl s type1 fixpoint_is_storage_coupon_api 
+  [(V_ref (ConstRefExtern r))] 
+  = Some (s, [V_num (ConstInt32 (bool_to_i32 (is_storage_coupon_api (to_handle r))))])"
+and
+  fixpoint_get_coupon_lhs_impl:
+  "host_func_apply_impl s type2 fixpoint_get_coupon_lhs 
+  [(V_ref (ConstRefExtern r))] 
+  = map_option (\<lambda>h. (s, [V_ref (ConstRefExtern (to_externref h))])) (get_coupon_lhs (to_handle r))" 
+and
+  fixpoint_get_coupon_rhs_impl:
+  "host_func_apply_impl s type2 fixpoint_get_coupon_rhs 
+  [(V_ref (ConstRefExtern r))] 
+  = map_option (\<lambda>h. (s, [V_ref (ConstRefExtern (to_externref h))])) (get_coupon_rhs (to_handle r))" 
+and
+  fixpoint_create_eq_coupon_impl:
+  "host_func_apply_impl s type3 fixpoint_create_eq_coupon
+  [(V_ref (ConstRefExtern r1)), (V_ref (ConstRefExtern r2))] 
+  = Some (s, [V_ref (ConstRefExtern (to_externref (create_eq_coupon (to_handle r1) (to_handle r2))))])"
 
 (* Helper lemmas for simplifying bool_to_i32 from the axiom statement *)
-lemma fixpoint_is_equal_correct_handle:
-  "is_equal h1 h2 \<longleftrightarrow> host_func_apply_impl s type0 fixpoint_is_equal 
-  [(V_ref (ConstRefExtern (to_externref h1))), (V_ref (ConstRefExtern (to_externref h2)))] = Some(s, [V_num (ConstInt32 (I32.int_of_nat 1))])"
-  using fixpoint_is_equal_impl bool_to_i32_true by auto
-
-lemma fixpoint_is_equal_correct_handle_neq:
-  "\<not>is_equal h1 h2 \<longleftrightarrow> host_func_apply_impl s type0 fixpoint_is_equal 
-  [(V_ref (ConstRefExtern (to_externref h1))), (V_ref (ConstRefExtern (to_externref h2)))] = Some(s, [V_num (ConstInt32 (I32.int_of_nat 0))])"
-  using fixpoint_is_equal_impl bool_to_i32_false by auto
-
 lemma fixpoint_is_equal_correct_externref:
   "is_equal (to_handle r1) (to_handle r2) \<longleftrightarrow> host_func_apply_impl s type0 fixpoint_is_equal 
   [(V_ref (ConstRefExtern r1)), (V_ref (ConstRefExtern r2))] = Some(s, [V_num (ConstInt32 (I32.int_of_nat 1))])"
@@ -76,5 +96,17 @@ lemma fixpoint_is_equal_correct_externref:
 lemma fixpoint_is_equal_correct_externref_neq:
   "\<not>is_equal (to_handle r1) (to_handle r2) \<longleftrightarrow> host_func_apply_impl s type0 fixpoint_is_equal 
   [(V_ref (ConstRefExtern r1)), (V_ref (ConstRefExtern r2))] = Some(s, [V_num (ConstInt32 (I32.int_of_nat 0))])"
-  using fixpoint_is_equal_correct_handle_neq fixpoint_is_equal_impl by auto
+  using bool_to_i32_false fixpoint_is_equal_impl by auto
+
+lemma fixpoint_is_storage_coupon_api_externref:
+  "is_storage_coupon_api (to_handle r) \<longleftrightarrow> host_func_apply_impl s type1
+   fixpoint_is_storage_coupon_api
+   [(V_ref (ConstRefExtern r))] = Some(s, [V_num (ConstInt32 (I32.int_of_nat 1))])"
+  using bool_to_i32_true fixpoint_is_storage_coupon_api_impl by auto
+
+lemma fixpoint_is_storage_coupon_api_externref_neq:
+  "\<not>is_storage_coupon_api (to_handle r) \<longleftrightarrow> host_func_apply_impl s type1
+   fixpoint_is_storage_coupon_api
+   [(V_ref (ConstRefExtern r))] = Some(s, [V_num (ConstInt32 (I32.int_of_nat 0))])"
+  using bool_to_i32_false fixpoint_is_storage_coupon_api_impl by auto
 end
