wasm-proofs/Wasm-Proof/Init.thy
@@ -2,15 +2,24 @@ theory Init
   imports Host
 begin
 
-definition init :: "s" where
- "init = 
+definition func_ret_idx :: nat where "func_ret_idx = 5"
+definition func_make_blob_coupon_idx :: nat where "func_make_blob_coupon_idx = 6"
+definition tab_coupons_idx :: nat where "tab_coupons_idx = 0"
+definition init :: "s" where "init = 
 \<lparr> funcs = 
 [(Func_host ([(T_ref T_ext_ref), (T_ref T_ext_ref)] _> [(T_num T_i32)]) (Host_func fixpoint_is_equal)),
+(Func_host ([(T_ref T_ext_ref)] _> [(T_num T_i32)]) (Host_func fixpoint_is_storage_coupon_api)),
+(Func_host ([(T_ref T_ext_ref)] _> [(T_ref T_ext_ref)]) (Host_func fixpoint_get_coupon_lhs)),
+(Func_host ([(T_ref T_ext_ref)] _> [(T_ref T_ext_ref)]) (Host_func fixpoint_get_coupon_rhs)),
+(Func_host ([(T_ref T_ext_ref), (T_ref T_ext_ref)] _> [(T_ref T_ext_ref)]) (Host_func fixpoint_create_eq_coupon)),
+
 (Func_native 
 \<lparr>types = [([(T_ref T_ext_ref), (T_ref T_ext_ref)] _> [(T_num T_i32)]),
+([(T_ref T_ext_ref)] _> [(T_num T_i32)]),
+([(T_ref T_ext_ref)] _> [(T_ref T_ext_ref)]),
 ([(T_ref T_ext_ref), (T_ref T_ext_ref)] _> [(T_ref T_ext_ref)])],
-funcs = [0, 1],
-tabs = [],
+funcs = [0, 1, 2, 3, 4, 5, 6],
+tabs = [0],
 mems = [],
 globs = [],
 elems = [],
@@ -23,8 +32,43 @@ datas = []
 (Call 0),
 (If (Tbv (Some (T_ref T_ext_ref)))
 [(Local_get 0)]
-[(Local_get 1)]) ]) ],
-tabs = [],
+[(Local_get 1)])]),
+(Func_native 
+\<lparr>types = [([(T_ref T_ext_ref), (T_ref T_ext_ref)] _> [(T_num T_i32)]),
+([(T_ref T_ext_ref)] _> [(T_num T_i32)]),
+([(T_ref T_ext_ref)] _> [(T_ref T_ext_ref)]),
+([(T_ref T_ext_ref), (T_ref T_ext_ref)] _> [(T_ref T_ext_ref)])],
+funcs = [0, 1, 2, 3, 4, 5, 6],
+tabs = [0],
+mems = [],
+globs = [],
+elems = [],
+datas = []
+\<rparr>
+([(T_ref T_ext_ref), (T_ref T_ext_ref)] _> [(T_ref T_ext_ref)])
+[(T_ref T_ext_ref)]
+[(EConstNum (ConstInt32 (Abs_i32 0))),
+(Table_get 0),
+(Local_set 2),
+(Local_get 2),
+(Call 1),
+(If (Tbv (Some (T_ref T_ext_ref)))
+[(Local_get 0),
+(Local_get 2),
+(Call 2),
+(Call 0),
+(Local_get 1),
+(Local_get 2),
+(Call 3),
+(Call 0),
+(Binop T_i32 (Binop_i And)),
+(If (Tbv (Some (T_ref T_ext_ref)))
+[(Local_get 0),
+(Local_get 1),
+(Call 4)]
+[Unreachable])]
+[Unreachable])])],
+tabs = [((T_tab \<lparr> l_min = 0, l_max = None\<rparr> T_ext_ref), [])],
 mems = [],
 globs = [],
 elems = [],
