wasm-proofs/Wasm-Proof/Wasm_Proof_Playground.thy
@@ -14,36 +14,45 @@ lemma sf:
   "int_eq (I32.int_of_nat 0) 0"
   by (simp add: I32.int_eq_def I32.int_of_nat_def int_eq_i32.abs_eq zero_i32_def)
 
+lemma convert_50_to_suc:
+"(50::nat) =
+  (Suc (Suc (Suc (Suc (Suc (Suc (Suc (Suc (Suc (Suc
+  (Suc (Suc (Suc (Suc (Suc (Suc (Suc (Suc (Suc (Suc
+  (Suc (Suc (Suc (Suc (Suc (Suc (Suc (Suc (Suc (Suc
+  (Suc (Suc (Suc (Suc (Suc (Suc (Suc (Suc (Suc (Suc
+  (Suc (Suc (Suc (Suc (Suc (Suc (Suc (Suc (Suc (Suc 0))))))))))))))))))))))))))))))))))))))))))))))))))"
+  by simp
+
 (* Given a fuel and depth that is enough to get to the result state, after run_iter, the result is a specific input argument *)
 lemma init_run_iter:
   assumes "is_equal (to_handle r1) (to_handle r2)"
-  shows "run_iter (Suc (Suc (Suc (Suc (Suc (Suc (Suc (Suc (Suc (Suc (Suc (Suc n)))))))))))) (Config (Suc n') init (Frame_context (Redex [(V_ref (ConstRefExtern r2)), (V_ref (ConstRefExtern r1))] [Invoke 1] []) [] 0 empty_frame) []) = 
+  shows "run_iter 50 (Config (Suc n') init (Frame_context (Redex [(V_ref (ConstRefExtern r2)), (V_ref (ConstRefExtern r1))] [Invoke func_ret_idx] []) [] 0 empty_frame) []) = 
      (let v_s = [V_ref (ConstRefExtern r1)]
      in (Config (Suc n')
          init
          (Frame_context (Redex v_s [] []) [] 0 empty_frame) [],
          RValue v_s))"
   using fixpoint_is_equal_correct_externref[of r1 r2 init] assms
-  by (auto split: cl.splits simp add: n_zeros_def app_f_v_s_local_get_def app_f_call_def sfunc_ind_def typeof_def typeof_num_def init_def app_v_s_if_def se tb_tf_def)
+  by (auto split: cl.splits simp add: convert_50_to_suc n_zeros_def app_f_v_s_local_get_def app_f_call_def sfunc_ind_def typeof_def typeof_num_def init_def app_v_s_if_def se tb_tf_def func_ret_idx_def)
 
 lemma init_run_iter_neq:
   assumes "\<not>is_equal (to_handle r1) (to_handle r2)"
-  shows "run_iter (Suc (Suc (Suc (Suc (Suc (Suc (Suc (Suc (Suc (Suc (Suc (Suc n)))))))))))) (Config (Suc n') init (Frame_context (Redex [(V_ref (ConstRefExtern r2)), (V_ref (ConstRefExtern r1))] [Invoke 1] []) [] 0 empty_frame) []) = 
+  shows "run_iter 50 (Config (Suc n') init (Frame_context (Redex [(V_ref (ConstRefExtern r2)), (V_ref (ConstRefExtern r1))] [Invoke func_ret_idx] []) [] 0 empty_frame) []) = 
      (let v_s = [V_ref (ConstRefExtern r2)]
      in (Config (Suc n')
          init
          (Frame_context (Redex v_s [] []) [] 0 empty_frame) [],
          RValue v_s))"
   using fixpoint_is_equal_correct_externref_neq[of r1 r2 init] assms
-  by (auto split: cl.splits simp add: n_zeros_def app_f_v_s_local_get_def app_f_call_def sfunc_ind_def typeof_def typeof_num_def init_def app_v_s_if_def sf tb_tf_def)
+  by (auto split: cl.splits simp add: convert_50_to_suc n_zeros_def app_f_v_s_local_get_def app_f_call_def sfunc_ind_def typeof_def typeof_num_def init_def app_v_s_if_def sf tb_tf_def func_ret_idx_def fixpoint_is_equal_impl)
 
 (* From the run_iter lemmas, one step out to the run_invoke lemmas *)
 lemma init_run_invoke:
   assumes "is_equal (to_handle r1) (to_handle r2)" 
-  shows "run_invoke_v (Suc (Suc (Suc (Suc (Suc (Suc (Suc (Suc (Suc (Suc (Suc (Suc 0))))))))))))
-   (Suc 0) (init, [(V_ref (ConstRefExtern r1)), (V_ref (ConstRefExtern r2))], 1) = (init, RValue [V_ref (ConstRefExtern r1)])"
+  shows "run_invoke_v 50
+   (Suc 0) (init, [(V_ref (ConstRefExtern r1)), (V_ref (ConstRefExtern r2))], func_ret_idx) = (init, RValue [V_ref (ConstRefExtern r1)])"
 proof -
-  have X: "run_iter (Suc (Suc (Suc (Suc (Suc (Suc (Suc (Suc (Suc (Suc (Suc (Suc 0)))))))))))) (Config (Suc 0) init (Frame_context (Redex [(V_ref (ConstRefExtern r2)), (V_ref (ConstRefExtern r1))] [Invoke 1] []) [] 0 empty_frame) []) = 
+  have X: "run_iter 50 (Config (Suc 0) init (Frame_context (Redex [(V_ref (ConstRefExtern r2)), (V_ref (ConstRefExtern r1))] [Invoke func_ret_idx] []) [] 0 empty_frame) []) = 
      (let v_s = [V_ref (ConstRefExtern r1)]
      in (Config (Suc 0)
          init
@@ -63,10 +72,10 @@ qed
 
 lemma init_run_invoke_neq:
   assumes "\<not>is_equal (to_handle r1) (to_handle r2)" 
-  shows "run_invoke_v (Suc (Suc (Suc (Suc (Suc (Suc (Suc (Suc (Suc (Suc (Suc (Suc 0))))))))))))
-   (Suc 0) (init, [(V_ref (ConstRefExtern r1)), (V_ref (ConstRefExtern r2))], 1) = (init, RValue [V_ref (ConstRefExtern r2)])"
+  shows "run_invoke_v 50
+   (Suc 0) (init, [(V_ref (ConstRefExtern r1)), (V_ref (ConstRefExtern r2))], func_ret_idx) = (init, RValue [V_ref (ConstRefExtern r2)])"
 proof -
-  have X: "run_iter (Suc (Suc (Suc (Suc (Suc (Suc (Suc (Suc (Suc (Suc (Suc (Suc 0)))))))))))) (Config (Suc 0) init (Frame_context (Redex [(V_ref (ConstRefExtern r2)), (V_ref (ConstRefExtern r1))] [Invoke 1] []) [] 0 empty_frame) []) = 
+  have X: "run_iter 50 (Config (Suc 0) init (Frame_context (Redex [(V_ref (ConstRefExtern r2)), (V_ref (ConstRefExtern r1))] [Invoke func_ret_idx] []) [] 0 empty_frame) []) = 
      (let v_s = [V_ref (ConstRefExtern r2)]
      in (Config (Suc 0)
          init
@@ -87,14 +96,273 @@ qed
 fun isabelle_func :: "handle \<Rightarrow> handle \<Rightarrow> handle" where
   "isabelle_func h1 h2 = (if (is_equal h1 h2) then h1 else h2)"
 
+
 (* Now we show that the function at index 1 is equivalent to the isabelle function such that there exists a fuel and depth such that for any pair of input handles, translating those to externrefs and invoking the function with the fuel and depth returns a result that is the same as translating the isabelle function output to an externref.*)
 lemma func_equiv:
   "\<exists>f d s.
    run_invoke_v f d 
    (init, 
    [V_ref (ConstRefExtern (to_externref h1)), 
-    V_ref (ConstRefExtern (to_externref h2))], 1) 
+    V_ref (ConstRefExtern (to_externref h2))], func_ret_idx) 
    = (s, RValue [V_ref (ConstRefExtern (to_externref (isabelle_func h1 h2)))])"
   by (metis init_run_invoke init_run_invoke_neq isabelle_func.simps to_handle_to_externref)
+
+fun make_blob_coupon_raw :: "handle list \<Rightarrow> handle \<Rightarrow> handle \<Rightarrow> handle option" where
+  "make_blob_coupon_raw (c # xs) l r =
+   (if (is_storage_coupon_api c) 
+    then (case (get_coupon_lhs c, get_coupon_rhs c) of
+     (Some l', Some r') \<Rightarrow> (if ( is_equal l l' \<and> is_equal r r') then Some (create_eq_coupon l r)
+                                                                else None)
+    | _ \<Rightarrow> None)
+    else None)"
+| "make_blob_coupon_raw [] l r = None"
+
+lemma mb_some:
+  assumes "make_blob_coupon_raw coupons l r = Some res"
+  shows "(\<exists>c xs l' r'. coupons = c # xs
+              \<and> is_storage_coupon_api c
+              \<and> get_coupon_lhs c = Some l'
+              \<and> get_coupon_rhs c = Some r'
+              \<and> is_equal l l'
+              \<and> is_equal r r'
+              \<and> res = (create_eq_coupon l r))"
+proof -
+  obtain c xs l' r' where 1: "coupons  = c # xs"
+                      and 2: "is_storage_coupon_api c"
+                      and 3: "get_coupon_lhs c = Some l'"
+                      and 4: "get_coupon_rhs c = Some r'"
+  by (metis assms is_coupon_lhs is_coupon_rhs is_storage_coupon_api_def make_blob_coupon_raw.elims option.simps(3))
+
+  then have "make_blob_coupon_raw coupons l r = 
+       (if (is_equal l l' \<and> is_equal r r') then Some (create_eq_coupon l r) else None)"
+    by (simp add: 1 2 3 4)
+
+  then show ?thesis
+    by (metis "1" "2" "3" "4" assms handy_if_lemma)
+qed
+
+lemma make_blob_coupon_raw_run_iter:
+  assumes "make_blob_coupon_raw coupons l r = Some res"
+  shows  "(run_invoke_v 50  (Suc 0)
+         (init\<lparr> tabs := (tabs init)[tab_coupons_idx := ((T_tab \<lparr> l_min = 0, l_max = None\<rparr> T_ext_ref), (map (\<lambda>c. (ConstRefExtern (to_externref c))) coupons))] \<rparr>,
+   [(V_ref (ConstRefExtern (to_externref l))), 
+         (V_ref (ConstRefExtern (to_externref r)))],
+        func_make_blob_coupon_idx) = 
+(init\<lparr> tabs := (tabs init)[tab_coupons_idx := ((T_tab \<lparr> l_min = 0, l_max = None\<rparr> T_ext_ref), (map (\<lambda>c. (ConstRefExtern (to_externref c))) coupons))] \<rparr>, RValue [V_ref (ConstRefExtern (to_externref (create_eq_coupon l r)))]))"
+proof -
+  obtain c xs l' r' where 1: "coupons = c # xs"
+                      and 2: "is_storage_coupon_api c"
+                      and 3: "get_coupon_lhs c = Some l'"
+                      and 4: "get_coupon_rhs c = Some r'"
+                      and 5: "is_equal l l'"
+                      and 6: "is_equal r r'"
+                      and 7: "res = (create_eq_coupon l r)"
+    using mb_some assms by blast
+
+  let ?state = " (init\<lparr> tabs := (tabs init)[tab_coupons_idx := ((T_tab \<lparr> l_min = 0, l_max = None\<rparr> T_ext_ref), (map (\<lambda>c. (ConstRefExtern (to_externref c))) coupons))] \<rparr> )"
+
+  let ?ce = "to_externref c"
+
+  have A: "nat_of_int (I32.lift0 0) < length coupons"
+    by (metis "1" Abs_fnat_hom_0 gr_zeroI impossible_Cons le0 zero zero_i32_def)
+
+  have B: "(coupons ! nat_of_int (I32.lift0 0)) = c"
+    using "1" nat_of_int_i32.abs_eq by auto
+
+  have C: "\<And>s. (host_func_apply_impl s type1 fixpoint_is_storage_coupon_api 
+    [V_ref (ConstRefExtern (to_externref c))] = Some (s, [V_num (ConstInt32 (I32.int_of_nat 1))]))"
+    using bool_to_i32_true fixpoint_is_storage_coupon_api_impl 2 by auto
+
+  have D: "(I32.int_and 1 1) = 1"
+    using I32.int_and_def by force
+  have D: "(int_and (I32.int_of_nat (Suc 0)) (I32.int_of_nat (Suc 0))) = (I32.int_of_nat 1)"
+    by (simp add: D I32.int_of_nat_def
+        int_and_i32.abs_eq)
+
+  show ?thesis
+    using A C[of ?state] 
+          fixpoint_get_coupon_lhs_impl[of ?state ?ce] 3 
+          fixpoint_get_coupon_rhs_impl[of ?state ?ce] 4
+          fixpoint_is_equal_correct_externref[of "to_externref l" "to_externref l'" ?state] 5
+          fixpoint_is_equal_correct_externref[of "to_externref r" "to_externref r'" ?state] 6
+          fixpoint_create_eq_coupon_impl[of ?state "to_externref l" "to_externref r"] 7
+    by (auto split: cl.splits simp add: convert_50_to_suc init_def func_make_blob_coupon_idx_def n_zeros_def bitzero_def tab_coupons_idx_def app_s_f_v_s_table_get_def stab_ind_def load_tabs1_def B
+    app_f_v_s_local_set_def app_f_v_s_local_get_def app_f_call_def sfunc_ind_def typeof_def typeof_num_def app_v_s_if_def se tb_tf_def typeof_ref_def app_v_s_binop_def app_binop_def app_binop_i_v_def app_binop_i_def D Let_def)
+qed
+
+
+lemma mb_some_rev:
+  assumes "(\<exists>c xs l' r'. coupons = c # xs
+              \<and> is_storage_coupon_api c
+              \<and> get_coupon_lhs c = Some l'
+              \<and> get_coupon_rhs c = Some r'
+              \<and> is_equal l l'
+              \<and> is_equal r r'
+              \<and> res = (create_eq_coupon l r))"
+  shows "make_blob_coupon_raw coupons l r = Some res"
+  using assms by fastforce
+
+lemma mb_none:
+  assumes "make_blob_coupon_raw coupons l r = None"
+  shows "(coupons = [] \<or>
+          (\<exists> c xs. coupons = c # xs \<and> \<not> is_storage_coupon_api c) \<or>
+          (\<exists> c xs l' r'. coupons = c # xs \<and> 
+                         is_storage_coupon_api c \<and> 
+                         get_coupon_lhs c = Some l' \<and>
+                         get_coupon_rhs c = Some r' \<and>
+                         \<not> is_equal l l') \<or>
+          (\<exists> c xs l' r'. coupons = c # xs \<and>
+                         is_storage_coupon_api c \<and>
+                         get_coupon_lhs c = Some l' \<and>
+                         get_coupon_rhs c = Some r' \<and>
+                         is_equal l l' \<and>
+                         \<not> is_equal r r'))"
+  by (metis assms if_Some_None_eq_None is_coupon_lhs is_coupon_rhs is_storage_coupon_api_def make_blob_coupon_raw.elims mb_some_rev)
+
+lemma make_blob_coupon_raw_run_invoke_none:
+  assumes "make_blob_coupon_raw coupons l r = None"
+  shows "\<exists>msg. run_invoke_v 50 (Suc 0) 
+        (init\<lparr> tabs := (tabs init)[tab_coupons_idx := ((T_tab \<lparr> l_min = 0, l_max = None\<rparr> T_ext_ref), (map (\<lambda>c. (ConstRefExtern (to_externref c))) coupons))] \<rparr>,
+        [(V_ref (ConstRefExtern (to_externref l))), 
+         (V_ref (ConstRefExtern (to_externref r)))],
+        func_make_blob_coupon_idx)
+        = (init\<lparr> tabs := (tabs init)[tab_coupons_idx := ((T_tab \<lparr> l_min = 0, l_max = None\<rparr> T_ext_ref), (map (\<lambda>c. (ConstRefExtern (to_externref c))) coupons))] \<rparr>, RTrap msg)"
+proof -
+  let ?A = "coupons = []"
+  let ?B = "(\<exists> c xs. coupons = c # xs \<and> \<not> is_storage_coupon_api c)"
+  let ?C = "(\<exists> c xs l' r'. coupons = c # xs \<and> 
+                              is_storage_coupon_api c \<and> 
+                              get_coupon_lhs c = Some l' \<and>
+                              get_coupon_rhs c = Some r' \<and>
+                              \<not> is_equal l l')"
+  let ?D = "(\<exists> c xs l' r'. coupons = c # xs \<and>
+                              is_storage_coupon_api c \<and>
+                              get_coupon_lhs c = Some l' \<and>
+                              get_coupon_rhs c = Some r' \<and>
+                              is_equal l l' \<and>
+                              \<not> is_equal r r')"
+
+  have assms: "?A \<or> ?B \<or> ?C \<or> ?D" using mb_none assms by auto
+
+  let ?state = "(init\<lparr> tabs := (tabs init)[tab_coupons_idx := ((T_tab \<lparr> l_min = 0, l_max = None\<rparr> T_ext_ref), (map (\<lambda>c. (ConstRefExtern (to_externref c))) coupons))] \<rparr> )"
+
+  let ?lhs = "run_invoke_v 50 (Suc 0) 
+        (?state,
+        [(V_ref (ConstRefExtern (to_externref l))), 
+         (V_ref (ConstRefExtern (to_externref r)))],
+        func_make_blob_coupon_idx)"
+
+  let ?f = "\<lparr>f_locs = [V_ref (ConstRefExtern (to_externref l)), V_ref (ConstRefExtern (to_externref r)), V_ref (bitzero_ref T_ext_ref)],
+           f_inst =
+             \<lparr>types =
+                [[T_ref T_ext_ref, T_ref T_ext_ref] _> [T_num T_i32], [T_ref T_ext_ref] _> [T_num T_i32], [T_ref T_ext_ref] _> [T_ref T_ext_ref],
+                 [T_ref T_ext_ref, T_ref T_ext_ref] _> [T_ref T_ext_ref]],
+                funcs = [0, Suc 0, 2, 3, 4, 5, 6], tabs = [0], mems = [], globs = [], elems = [], datas = []\<rparr>\<rparr>"
+
+  show ?thesis
+    using assms
+  proof
+    assume "?A"
+    then have 1: "\<not> nat_of_int (I32.lift0 0) < length coupons" by auto
+
+    have "?lhs = (?state, RTrap STR ''table_get'')"
+      using 1
+      by (auto split: cl.splits simp add: convert_50_to_suc init_def func_make_blob_coupon_idx_def n_zeros_def bitzero_def tab_coupons_idx_def app_s_f_v_s_table_get_def stab_ind_def load_tabs1_def)
+    then show "\<exists>msg. ?lhs = (?state, RTrap msg)" by blast
+  next
+    assume "?B \<or> ?C \<or> ?D"
+    then show "\<exists>msg. ?lhs = (?state, RTrap msg)"
+    proof
+      assume ?B
+      then obtain c xs where 1: "coupons = c # xs" and 2: "\<not> is_storage_coupon_api c" by auto
+
+      have "?lhs = (?state, RTrap STR ''unreachable'')"
+        using fixpoint_is_storage_coupon_api_externref_neq[of "to_externref c" ?state] 2
+        by (auto split: cl.splits simp add: convert_50_to_suc init_def func_make_blob_coupon_idx_def n_zeros_def bitzero_def tab_coupons_idx_def app_s_f_v_s_table_get_def stab_ind_def load_tabs1_def app_f_v_s_local_set_def app_f_v_s_local_get_def app_f_call_def sfunc_ind_def typeof_def typeof_num_def app_v_s_if_def se tb_tf_def typeof_ref_def app_v_s_binop_def app_binop_def app_binop_i_v_def app_binop_i_def 1 nat_of_int_i32.abs_eq sf)
+      then show "\<exists>msg. ?lhs = (?state, RTrap msg)" by blast
+    next
+      assume "?C \<or> ?D"
+      then show "\<exists>msg. ?lhs = (?state, RTrap msg)"
+      proof
+        assume ?C
+        then obtain c xs l' r' where 1: "coupons = c # xs"
+                                 and 2: "is_storage_coupon_api c"
+                                 and 3: "get_coupon_lhs c = Some l'"
+                                 and 4: "get_coupon_rhs c = Some r'"
+                                 and 5: "\<not> is_equal l l'"
+          by blast
+
+        have 6: "I32.int_and 0 0 = 0"
+          using I32.int_and_def by force
+        have 6: "(int_and (I32.int_of_nat 0) (I32.int_of_nat 0)) = (I32.int_of_nat 0)"
+          by (simp add: 6 I32.int_of_nat_def int_and_i32.abs_eq)
+
+        have 7: "I32.int_and 0 1 = 0"
+          using I32.int_and_def by force
+        have 7: "(int_and (I32.int_of_nat 0) (I32.int_of_nat (Suc 0))) = (I32.int_of_nat 0)"
+          by (simp add: 7 I32.int_of_nat_def int_and_i32.abs_eq)
+
+        have "?lhs = (?state, RTrap STR ''unreachable'')"
+          using fixpoint_is_storage_coupon_api_externref[of "to_externref c" ?state] 2
+          fixpoint_get_coupon_lhs_impl[of ?state "to_externref c"] 3
+          fixpoint_get_coupon_rhs_impl[of ?state "to_externref c"] 4
+          fixpoint_is_equal_correct_externref_neq[of "to_externref l" "to_externref l'" ?state] 5
+          fixpoint_is_equal_correct_externref[of "to_externref r" "to_externref r'" ?state]
+          fixpoint_is_equal_correct_externref_neq[of "to_externref r" "to_externref r'" ?state]
+      
+          apply (auto split: cl.splits simp add: convert_50_to_suc init_def func_make_blob_coupon_idx_def n_zeros_def bitzero_def tab_coupons_idx_def app_s_f_v_s_table_get_def stab_ind_def load_tabs1_def app_f_v_s_local_set_def app_f_v_s_local_get_def app_f_call_def sfunc_ind_def typeof_def typeof_num_def app_v_s_if_def se tb_tf_def typeof_ref_def app_v_s_binop_def app_binop_def app_binop_i_v_def app_binop_i_def 1 nat_of_int_i32.abs_eq sf)
+          apply (cases "is_equal r r'")
+          apply (auto split: cl.splits simp add: convert_50_to_suc init_def func_make_blob_coupon_idx_def n_zeros_def bitzero_def tab_coupons_idx_def app_s_f_v_s_table_get_def stab_ind_def load_tabs1_def app_f_v_s_local_set_def app_f_v_s_local_get_def app_f_call_def sfunc_ind_def typeof_def typeof_num_def app_v_s_if_def se tb_tf_def typeof_ref_def app_v_s_binop_def app_binop_def app_binop_i_v_def app_binop_i_def 1 nat_of_int_i32.abs_eq sf 6 7)
+          done
+          
+        then show "\<exists>msg. ?lhs = (?state, RTrap msg)" by blast
+      next
+        assume ?D
+        then obtain c xs l' r' where 1: "coupons = c # xs"
+                                 and 2: "is_storage_coupon_api c"
+                                 and 3: "get_coupon_lhs c = Some l'"
+                                 and 4: "get_coupon_rhs c = Some r'"
+                                 and 5: "is_equal l l'"
+                                 and 6: "\<not> is_equal r r'"
+          by blast
+        
+        have 7: "I32.int_and 1 0 = 0"
+          using I32.int_and_def by force
+        have 7: "(int_and (I32.int_of_nat (Suc 0)) (I32.int_of_nat 0)) = (I32.int_of_nat 0)"
+          by (simp add: 7 I32.int_of_nat_def int_and_i32.abs_eq)
+        
+        have "?lhs = (?state, RTrap STR ''unreachable'')"
+          using fixpoint_is_storage_coupon_api_externref[of "to_externref c" ?state] 2
+          fixpoint_get_coupon_lhs_impl[of ?state "to_externref c"] 3
+          fixpoint_get_coupon_rhs_impl[of ?state "to_externref c"] 4
+          fixpoint_is_equal_correct_externref[of "to_externref l" "to_externref l'" ?state] 5
+          fixpoint_is_equal_correct_externref_neq[of "to_externref r" "to_externref r'" ?state] 6
+        
+          by (auto split: cl.splits simp add: convert_50_to_suc init_def func_make_blob_coupon_idx_def n_zeros_def bitzero_def tab_coupons_idx_def app_s_f_v_s_table_get_def stab_ind_def load_tabs1_def app_f_v_s_local_set_def app_f_v_s_local_get_def app_f_call_def sfunc_ind_def typeof_def typeof_num_def app_v_s_if_def se tb_tf_def typeof_ref_def app_v_s_binop_def app_binop_def app_binop_i_v_def app_binop_i_def 1 nat_of_int_i32.abs_eq sf 7)
+        
+        then show "\<exists>msg. ?lhs = (?state, RTrap msg)" by blast
+      qed
+    qed
+  qed
+qed
+
+lemma make_blob_coupon_raw_equiv:
+  "(\<And>res. 
+   (make_blob_coupon_raw coupons l r = Some res \<longrightarrow>
+      (\<exists>f d s.
+      run_invoke_v f d
+      (init\<lparr> tabs := (tabs init)[tab_coupons_idx := ((T_tab \<lparr> l_min = 0, l_max = None\<rparr> T_ext_ref), (map (\<lambda>c. (ConstRefExtern (to_externref c))) coupons))] \<rparr>,
+      [V_ref (ConstRefExtern (to_externref l)), 
+       V_ref (ConstRefExtern (to_externref r))], func_make_blob_coupon_idx) 
+      = (s, RValue [V_ref (ConstRefExtern (to_externref res))]))) \<and> 
+
+   (make_blob_coupon_raw coupons l r = None \<longrightarrow>
+      (\<exists>f d s msg.
+      run_invoke_v f d 
+      (init\<lparr> tabs := (tabs init)[tab_coupons_idx := ((T_tab \<lparr> l_min = 0, l_max = None\<rparr> T_ext_ref), (map (\<lambda>c. (ConstRefExtern (to_externref c))) coupons))] \<rparr>,
+      [V_ref (ConstRefExtern (to_externref l)), 
+       V_ref (ConstRefExtern (to_externref r))], func_make_blob_coupon_idx) 
+      = (s, RTrap msg))))"
+  by (metis (lifting) make_blob_coupon_raw_run_invoke_none make_blob_coupon_raw_run_iter mb_some)
 
 end
